Cslib/Logics/Propositional/Metalogic/Soundness.lean
@@ -69,7 +69,7 @@ theorem prop_soundness
   match d with
   | .ax _ ψ h_ax => exact prop_axiom_sound h_ax v
   | .assumption _ ψ h_mem => exact h_ctx ψ h_mem
-  | .modus_ponens _ ψ χ d₁ d₂ =>
+  | .modusPonens _ ψ χ d₁ d₂ =>
     exact prop_soundness d₁ v h_ctx
       (prop_soundness d₂ v h_ctx)
   | .weakening Γ' Δ ψ d' h_sub =>
